add SOCv1, typical behavior of shift-overflow counters, solved 283 TMs

verify/BinaryCounterFull.v
@@ -15,8 +15,374 @@ Inductive full: positive -> Prop :=
 | full_S x: full x -> full (xI x)
 .
 
+Fixpoint pow2(n:nat):positive :=
+match n with
+| O => xH
+| S n0 => xO (pow2 n0)
+end.
+
+Fixpoint pow2'(n:nat):positive :=
+match n with
+| O => xH
+| S n0 => xI (pow2' n0)
+end.
+
+Fixpoint log2(n:positive):nat :=
+match n with
+| xH => O
+| xI n0 => S (log2 n0)
+| xO n0 => S (log2 n0)
+end.
+
+Fixpoint ctz(n:positive):nat :=
+match n with
+| xO n0 => S (ctz n0)
+| _ => O
+end.
+
+Fixpoint shr(n:positive)(k:nat){struct k}:N :=
+match k with
+| O => Npos n
+| S k0 =>
+  match n with
+  | xH => N0
+  | xO n0 => shr n0 k0
+  | xI n0 => shr n0 k0
+  end
+end.
+
+
 
 Open Scope positive.
+
+Lemma full_iff_pow2' n:
+  full n <->
+  n = pow2' (log2 n).
+Proof.
+  split; intro.
+  - induction n.
+    + inversion H; subst.
+      specialize (IHn H1).
+      cbn. congruence.
+    + inversion H.
+    + reflexivity.
+  - induction n.
+    + cbn in H.
+      inversion H; subst.
+      specialize (IHn H1).
+      constructor.
+      congruence.
+    + inversion H.
+    + constructor.
+Qed.
+
+Lemma not_full_log2_S {n} (Hnf:not_full n):
+  log2 (Pos.succ n) = log2 n.
+Proof.
+  induction Hnf; cbn; auto.
+Qed.
+
+Lemma pow2'_spec n:
+  Pos.succ (pow2' n) = pow2 (S n).
+Proof.
+  induction n; cbn; auto.
+  rewrite IHn.
+  reflexivity.
+Qed.
+
+Definition rest(n:positive):N :=
+  Npos (pow2' (log2 n)) - (Npos n).
+
+Lemma pow2'_log2_ge n:
+  (pow2' (log2 n) >= n)%positive.
+Proof.
+  induction n; cbn; lia.
+Qed.
+
+Lemma rest_mul2 n:
+  (rest (n~0) = (rest n)*2+1)%N.
+Proof.
+  unfold rest.
+  cbn[log2].
+  cbn[pow2'].
+  pose proof (pow2'_log2_ge n) as H.
+  lia.
+Qed.
+
+Lemma rest_mul_pow2 n i:
+  (rest (n*(pow2 i))+1 = ((rest n)+1)*(Npos (pow2 i)))%N.
+Proof.
+  induction i.
+  - cbn[pow2].
+    rewrite N.mul_1_r.
+    rewrite Pos.mul_1_r.
+    reflexivity.
+  - cbn[pow2].
+    rewrite POrderedType.Positive_as_OT.mul_xO_r.
+    pose proof (rest_mul2 (n*pow2 i)) as H.
+    lia.
+Qed.
+
+Lemma full_iff_rest_eq0 n:
+  full n <-> rest n = N0.
+Proof.
+  rewrite full_iff_pow2'.
+  unfold rest.
+  pose proof (pow2'_log2_ge n).
+  lia.
+Qed.
+
+Lemma not_full_iff_pow2' n:
+  not_full n <-> (n < pow2' (log2 n))%positive.
+Proof.
+  induction n.
+  - split; intro H.
+    + inversion H; subst.
+      rewrite IHn in H1. cbn. lia.
+    + constructor.
+      rewrite IHn.
+      cbn in H. lia.
+  - split; intro H.
+    + cbn.
+      pose proof (pow2'_log2_ge n). lia.
+    + constructor.
+  - cbn.
+    split; intro H.
+    + inversion H; subst.
+    + lia.
+Qed.
+
+Lemma full_iff_rest n:
+  full n <-> rest n = N0.
+Proof.
+  rewrite full_iff_pow2'.
+  unfold rest.
+  pose proof (pow2'_log2_ge n) as H.
+  lia.
+Qed.
+
+Lemma not_full_iff_rest n:
+  not_full n <-> rest n <> N0.
+Proof.
+  rewrite not_full_iff_pow2'.
+  unfold rest.
+  lia.
+Qed.
+
+Lemma rest_S n:
+  rest n <> N0 ->
+  ((rest (Pos.succ n)) + 1)%N = rest n.
+Proof.
+  intro H.
+  unfold rest.
+  rewrite <-not_full_iff_rest in H.
+  rewrite (not_full_log2_S H).
+  rewrite not_full_iff_pow2' in H.
+  lia.
+Qed.
+
+Lemma rest_pow2_add n i x:
+  (n*(pow2 i) <= x < (n+1)*(pow2 i))%positive ->
+  ((rest n)*(Npos (pow2 i)) <= rest x < (rest n + 1)*(Npos (pow2 i)))%N.
+Proof.
+  generalize dependent x.
+  unfold rest.
+  induction i; intros.
+  - cbn in H.
+    assert (n=x) as E by lia.
+    subst.
+    cbn[pow2]. lia.
+  - destruct x.
+    + cbn[pow2].
+      cbn[log2]. cbn[pow2'].
+      cbn[pow2] in H.
+      specialize (IHi x). lia.
+    + cbn[pow2].
+      cbn[log2]. cbn[pow2'].
+      cbn[pow2] in H.
+      specialize (IHi x). lia.
+    + cbn in H. lia.
+Qed.
+
+Lemma not_empty_pow2_add n i x:
+  (n*(pow2 i) <= x < (n+1)*(pow2 i))%positive ->
+  pow2 (log2 n) < n ->
+  pow2 (log2 x) < x.
+Proof.
+  generalize dependent x.
+  unfold rest.
+  induction i; intros.
+  - cbn in H.
+    assert (n=x) as E by lia.
+    subst.
+    cbn[pow2]. lia.
+  - destruct x.
+    + cbn[log2]. cbn[pow2].
+      cbn[pow2'].
+      cbn[pow2] in H.
+      specialize (IHi x). lia.
+    + cbn[log2]. cbn[pow2].
+      cbn[pow2'].
+      cbn[pow2] in H.
+      specialize (IHi x). lia.
+    + cbn in H. lia.
+Qed.
+
+Lemma le_pow2a a b c d:
+  (b * N.pos (pow2 (c + (S d))) <= a)%N ->
+  (b*2 <= a)%N.
+Proof.
+  intro H.
+  rewrite Nat.add_comm in H.
+  cbn in H.
+  remember (N.pos (pow2 (d + c))~0) as c1.
+  assert (2<=c1)%N as H0 by lia.
+  pose proof (N.mul_le_mono_l _ _ b H0).
+  lia.
+Qed.
+
+Lemma log2_pow2 x:
+  log2 (pow2 x) = x.
+Proof.
+  induction x; cbn; auto.
+Qed.
+
+Lemma rest_pow2 x:
+  (rest (pow2 x) + 1 = Npos (pow2 x))%N.
+Proof.
+  induction x.
+  - reflexivity.
+  - cbn[pow2].
+    rewrite rest_mul2.
+    lia.
+Qed.
+
+Lemma split_bound m:
+  ((rest (pow2 (ctz m)) + 1) * 2 + shr m (S (ctz m)) <= (Npos m)*2)%N.
+Proof.
+  rewrite rest_pow2.
+  induction m.
+  - cbn[ctz].
+    cbn[pow2].
+    cbn[shr].
+    lia.
+  - cbn[ctz].
+    cbn[pow2].
+    remember (S (ctz m)) as c1.
+    cbn[shr].
+    lia.
+  - cbn; lia.
+Qed.
+
+Lemma split_bound' n l:
+  (2 <= n*2 < pow2 l)%positive ->
+  ((N.pos (pow2 (ctz n)))*4 + shr n (S (ctz n)) <= N.pos (pow2 l))%N.
+Proof.
+  generalize dependent n.
+  induction l; intros.
+  1: cbn in H; lia.
+  cbn in H.
+  destruct l as [|l].
+  1: cbn in H; lia.
+  cbn in H.
+  destruct n.
+  3: cbn; lia.
+  1: cbn[ctz]; cbn[shr]; cbn[pow2]; lia.
+  cbn[ctz]. cbn[pow2].
+  remember (S (ctz n)) as c1.
+  cbn[shr].
+  subst c1.
+  specialize (IHl n).
+  cbn[pow2] in IHl.
+  lia.
+Qed.
+
+
+Lemma rest_mul2add1 n:
+  (rest (n~1) = rest n * 2)%N.
+Proof.
+  replace (n~1) with (Pos.succ (n~0)) by lia.
+  assert (not_full (n~0))%positive as nf by constructor.
+  rewrite not_full_iff_rest in nf.
+  pose proof (rest_S (n~0) nf) as H3.
+  pose proof (rest_mul2 n).
+  lia.
+Qed.
+
+Lemma rest_le n:
+  (rest n <= rest (pow2 (log2 n)))%N.
+Proof.
+  induction n.
+  - assert (n~1 = Pos.succ (n~0))%positive as E by lia.
+    rewrite E.
+    assert (not_full (n~0))%positive as nf by constructor.
+    rewrite not_full_log2_S; auto.
+    rewrite not_full_iff_rest in nf.
+    pose proof (rest_S (n~0) nf) as H3.
+    assert (rest n~0 <= rest (pow2 (log2 n~0)))%N. {
+      rewrite rest_mul2.
+      cbn[log2].
+      pose proof (rest_pow2 (log2 n)) as H.
+      pose proof (rest_pow2 (S (log2 n))) as H0.
+      cbn[pow2].
+      cbn[pow2] in H0.
+      lia.
+    }
+    lia.
+  - rewrite rest_mul2.
+    cbn[log2].
+    pose proof (rest_pow2 (log2 n)) as H.
+    pose proof (rest_pow2 (S (log2 n))) as H0.
+    cbn[pow2].
+    cbn[pow2] in H0.
+    lia.
+  - cbn; lia.
+Qed.
+
+Lemma neq1_pow2_log2 k:
+  (k<>1 -> pow2 (log2 k) <> 1)%positive.
+Proof.
+  destruct k; cbn; intro H; lia.
+Qed.
+
+Lemma not_empty_rest_iff n:
+  pow2 (log2 n) < n <->
+  (rest n < rest (pow2 (log2 n)))%N.
+Proof.
+  split; intro H.
+  - unfold rest.
+    pose proof (pow2'_log2_ge n).
+    rewrite log2_pow2.
+    lia.
+  - unfold rest in H.
+    pose proof (pow2'_log2_ge n).
+    rewrite log2_pow2 in H.
+    lia.
+Qed.
+
+Lemma not_empty_rest_pow2_add n i x:
+  (n*(pow2 i) <= x < (n+1)*(pow2 i))%positive ->
+  (rest n < rest (pow2 (log2 n)) ->
+  rest x < rest (pow2 (log2 x)))%N.
+Proof.
+  intros H H0.
+  rewrite <-not_empty_rest_iff.
+  rewrite <-not_empty_rest_iff in H0.
+  eapply not_empty_pow2_add; eauto.
+Qed.
+
+Lemma rest_S_not_empty k:
+  (rest k <> 0)%N ->
+  (rest (Pos.succ k) < rest (pow2 (log2 (Pos.succ k))))%N.
+Proof.
+  intro H.
+  pose proof (rest_S _ H).
+  rewrite <-not_full_iff_rest in H.
+  rewrite not_full_log2_S; auto.
+  pose proof (rest_le k).
+  lia.
+Qed.
+
 
 Lemma full_iff n:
   full n <->
@@ -118,6 +484,14 @@ Lemma full_S__not_full n:
 Proof.
   intro Hf.
   induction Hf; cbn; constructor.
+Qed.
+
+Lemma full_cases n:
+  {full n} + {not_full n}.
+Proof.
+  destruct (is_full n) eqn:E.
+  - rewrite <-is_full_spec in E; auto.
+  - rewrite <-is_full_spec' in E; auto.
 Qed.
 
 Close Scope positive.
