verify/BinaryCounter.v
@@ -1,0 +1,188 @@
+From BusyCoq Require Import Individual62.
+From BusyCoq Require Import BinaryCounterFull.
+Require Import ZArith.
+Require Import Lia.
+
+Section BinaryCounter.
+Open Scope list.
+
+Hypothesis d0 d1:list Sym.
+Hypothesis d1a:side.
+Fixpoint BinaryCounter (n:positive) :=
+match n with
+| xH => d1a
+| xI n0 => d1 *> (BinaryCounter n0)
+| xO n0 => d0 *> (BinaryCounter n0)
+end.
+
+Definition BinaryCounter_0 (n:N) :=
+match n with
+| N0 => const 0
+| Npos n0 => BinaryCounter n0
+end.
+
+Lemma not_full_Inc {n} (Hnf:not_full n):
+  exists s i,
+  BinaryCounter n = d1^^i *> d0 *> s /\
+  BinaryCounter (Pos.succ n) = d0^^i *> d1 *> s.
+Proof.
+  induction Hnf.
+  - exists (BinaryCounter x) O.
+    auto.
+  - destruct IHHnf as [s [i [H0 H1]]].
+    exists s (S i).
+    cbn.
+    simpl_tape.
+    split; congruence.
+Qed.
+
+Lemma full_Overflow {n} (Hf:full n):
+  exists i,
+  BinaryCounter n = d1^^i *> d1a /\
+  BinaryCounter (Pos.succ n) = d0^^(S i) *> d1a /\
+  (n+1)%positive = (2^Pos.of_succ_nat i)%positive.
+Proof.
+  induction Hf.
+  - exists O.
+    repeat split; auto.
+    cbn. simpl_tape.
+    reflexivity.
+  - destruct IHHf as [i [H0 [H1 H2]]].
+    exists (S i).
+    cbn.
+    simpl_tape.
+    rewrite <-H0.
+    repeat split; auto.
+    + rewrite H1.
+      simpl_tape.
+      reflexivity.
+    + rewrite Pos.pow_succ_r. lia.
+Qed.
+
+Lemma Counter_pow2 n:
+  BinaryCounter (pow2 n) =
+  d0^^n *> d1a.
+Proof.
+  induction n; cbn; auto.
+  rewrite IHn,Str_app_assoc.
+  reflexivity.
+Qed.
+
+Lemma Counter_pow2' n:
+  BinaryCounter (pow2' n) =
+  d1^^n *> d1a.
+Proof.
+  induction n; cbn; auto.
+  rewrite IHn,Str_app_assoc.
+  reflexivity.
+Qed.
+
+Lemma Counter_shr_S_ctz n:
+  d1a = d1 *> const 0 ->
+  BinaryCounter_0 (Npos n) =
+  d0^^(ctz n) *> d1 *> BinaryCounter_0 (shr n (S (ctz n))).
+Proof.
+  intro H.
+  induction n; cbn; auto.
+  cbn in IHn.
+  rewrite IHn.
+  simpl_tape.
+  reflexivity.
+Qed.
+
+Lemma BinaryCounter_0_d0 n:
+  BinaryCounter_0 (Npos (n~0)) =
+  d0 *> BinaryCounter_0 (Npos n).
+Proof.
+  reflexivity.
+Qed.
+
+Lemma BinaryCounter_0_d1 n:
+  BinaryCounter_0 (Npos (n~1)) =
+  d1 *> BinaryCounter_0 (Npos n).
+Proof.
+  reflexivity.
+Qed.
+
+Hypothesis tm:TM.
+
+Hypothesis QL QR:Q.
+Hypothesis qL qR:list Sym.
+
+Local Notation "l <| r" :=
+  (l <{{QL}} qL *> r) (at level 30).
+
+Local Notation "l |> r" :=
+  (l <* qR {{QR}}> r) (at level 30).
+
+Lemma LInc:
+  (forall l r n,
+    l <* d0 <* d1^^n <| r -[ tm ]->+
+    l <* d1 <* d0^^n |> r) ->
+  forall n (Hnf:not_full n) r,
+    BinaryCounter n <| r -[ tm ]->+
+    BinaryCounter (Pos.succ n) |> r.
+Proof.
+  intros.
+  destruct (not_full_Inc Hnf) as [s [i [H0 H1]]].
+  rewrite H0,H1.
+  simpl_tape.
+  apply H.
+Qed.
+
+Lemma RInc:
+  (forall l r n,
+    l |> d1^^n *> d0 *> r -[ tm ]->+
+    l <| d0^^n *> d1 *> r) ->
+  forall n (Hnf:not_full n) l,
+    l |> BinaryCounter n -[ tm ]->+
+    l <| BinaryCounter (Pos.succ n).
+Proof.
+  intros.
+  destruct (not_full_Inc Hnf) as [s [i [H0 H1]]].
+  rewrite H0,H1.
+  simpl_tape.
+  apply H.
+Qed.
+
+Lemma RInc_0:
+  (forall l r n,
+    l |> d1^^n *> d0 *> r -[ tm ]->+
+    l <| d0^^n *> d1 *> r) ->
+  d1a = d1 *> const 0 ->
+  d0 *> const 0 = const 0 ->
+  forall n l,
+    l |> BinaryCounter_0 n -[ tm ]->+
+    l <| BinaryCounter_0 (N.succ n).
+Proof.
+  intros.
+  destruct n as [|n].
+  - cbn[BinaryCounter_0].
+    rewrite <-H1.
+    change (d0 *> const 0) with (d1^^0 *> d0 *> const 0).
+    follow10 H.
+    cbn.
+    rewrite H0.
+    finish.
+  - destruct (is_full n) eqn:E.
+    + rewrite <-is_full_spec in E.
+      cbn.
+      destruct (full_Overflow E) as [i [H2 [H3 H4]]].
+      rewrite H2,H3.
+      rewrite H0.
+      rewrite lpow_shift'.
+      specialize (H l (const 0) (S i)).
+      cbn in H. cbn.
+      gen H.
+      simpl_tape.
+      rewrite H1.
+      tauto.
+    + rewrite <-is_full_spec' in E.
+      destruct (not_full_Inc E) as [s [i [H2 H3]]].
+      cbn.
+      rewrite H2,H3.
+      apply H.
+Qed.
+
+
+End BinaryCounter.
