verify/SOCv1.v
@@ -1,0 +1,738 @@
+From BusyCoq Require Import Individual62.
+From BusyCoq Require Import BinaryCounterFull.
+From BusyCoq Require Import BinaryCounter.
+Require Import Lia.
+Require Import ZArith.
+Require Import String.
+Require Import List.
+
+
+Section SOCv1.
+
+Hypothesis tm: TM.
+
+Notation "c --> c'" := (c -[ tm ]-> c')   (at level 40).
+Notation "c -->* c'" := (c -[ tm ]->* c') (at level 40).
+Notation "c -->+ c'" := (c -[ tm ]->+ c') (at level 40).
+
+Hypothesis QL QR:Q.
+Hypothesis m0 m1:list Sym.
+Hypothesis v0: nat.
+Hypothesis ls0 ls1 ls2: list nat.
+Hypothesis ls3 ls4 ls5: list nat.
+
+Hypothesis k_init:positive.
+Hypothesis n_init:N.
+
+Notation "l <| r" :=
+  (l <{{QL}} m0 *> r) (at level 30).
+
+Notation "l |> r" :=
+  (l <* m1 {{QR}}> r) (at level 30).
+
+Definition d0 := [0;1].
+Definition d1 := [1;1].
+Definition d1' := [1;1].
+Definition d1a := [1].
+
+Hypothesis LInc:
+  forall (l r:side) n,
+    l <* d0 <* d1^^n <| r -->+
+    l <* d1 <* d0^^n |> r.
+
+Definition rd0 := [0;0;0;0].
+Definition rd1 := [1;0;0;0].
+
+Hypothesis RInc:
+  forall (l r:side) n,
+    l |> rd1^^n *> [0] *> r -->+
+    l <| rd0^^n *> [1] *> r.
+
+Definition r0 := [1].
+Definition r1 := [1].
+
+Lemma L_rotate:
+  d1' = r0 ++ r1.
+Proof.
+  reflexivity.
+Qed.
+
+Lemma L_rotate':
+  d1' = r1 ++ r0.
+Proof.
+  reflexivity.
+Qed.
+
+Definition to_Ldigit(n:nat):=
+match n with
+| O => d0
+| _ => d1
+end.
+
+Hypothesis LOverflow_0:
+  forall r n,
+    const 0 <* d1a <* d1^^(n+1) <| rd0 *> r -->+
+    const 0 <* d1a <* d0^^(n+1)|> rd1 *> [0] *> r.
+
+Hypothesis LOverflow_1:
+  forall r n,
+    const 0 <* d1a <* d1^^(n+1) <| rd1 *> r -->+
+    const 0 <* d1a <* d0^^(n+1) <* (to_Ldigit v0) |> [0;0;0] *> r.
+
+Hypothesis Hls02:
+  length ls0 + length ls2 = 2.
+Hypothesis Hls1:
+  length ls1 = 2.
+Hypothesis Hls35:
+  length ls3 + length ls5 = 1%nat.
+Hypothesis Hls4:
+  length ls4 = 2.
+
+Hypothesis ROverflow_1001:
+  forall l r n,
+    l |> rd1^^n *> [1;0;0;1] *> r -->+
+    l <* (flat_map to_Ldigit (ls0++ls1^^n++ls2)) |> r.
+
+Hypothesis ROverflow_11:
+  forall l r n,
+    l |> rd1^^n *> [1;1] *> r -->+
+    l <* (flat_map to_Ldigit (ls3++ls4^^n++ls5)) |> r.
+
+
+Definition LC n :=
+  BinaryCounter d0 d1 (d1a *> const 0) n.
+
+Definition RC n :=
+  BinaryCounter_0 rd0 rd1 (rd1 *> const 0) n.
+
+Definition RC0 n m :=
+  BinaryCounter rd0 rd1 ([0] *> rd1 *> RC m) n.
+
+Definition RC1 n m :=
+  BinaryCounter rd0 rd1 ([1] *> rd1 *> RC m) n.
+
+Definition RC2 n m :=
+  BinaryCounter rd0 rd1 ([0;0;0] *> rd1 *> RC m) n.
+
+Definition RC3 n m :=
+  BinaryCounter rd0 rd1 ([1;0;0] *> rd1 *> RC m) n.
+
+Lemma rotate_000 n r:
+  rd0^^n *> [0;0;0] *> r =
+  [0;0;0] *> rd0^^n *> r.
+Proof.
+  induction n.
+  - reflexivity.
+  - cbn[lpow].
+    repeat rewrite Str_app_assoc.
+    rewrite IHn.
+    reflexivity.
+Qed.
+
+Lemma rotate_0 n r:
+  rd0^^n *> [0] *> r =
+  [0] *> rd0^^n *> r.
+Proof.
+  induction n.
+  - reflexivity.
+  - cbn[lpow].
+    repeat rewrite Str_app_assoc.
+    rewrite IHn.
+    reflexivity.
+Qed.
+
+Lemma LC_shl n ls:
+  (exists n0,
+  flat_map to_Ldigit ls *> LC n = LC n0 /\
+  n*(pow2 (length ls)) <= n0 /\
+  n0 < (n+1)*(pow2 (length ls)))%positive.
+Proof.
+  induction ls.
+  - cbn. exists n. split; auto; lia.
+  - cbn. repeat rewrite Str_app_assoc.
+    destruct IHls as [n0 [H0 [H1 H2]]].
+    rewrite H0.
+    destruct a as [|a].
+    + exists (xO n0).
+      split; auto; lia.
+    + exists (xI n0).
+      split; auto; lia.
+Qed.
+
+
+
+
+Lemma LC_Inc n (Hnf:not_full n) r:
+  LC n <| r -->+
+  LC (Pos.succ n) |> r.
+Proof.
+  apply BinaryCounter.LInc; assumption.
+Qed.
+
+Lemma LC_Overflow_0' n:
+  pow2' n <> xH ->
+  LC (pow2' n) <| RC 0 -->+
+  LC (pow2 n) |> RC 1.
+Proof.
+  intro H.
+  destruct n as [|n].
+  1: cbn in H; lia.
+  replace (S n) with (n+1) by lia.
+  unfold LC.
+  rewrite Counter_pow2,Counter_pow2'.
+  replace (RC 0) with (rd0 *> const 0). 2:{
+    cbn.
+    repeat rewrite <-const_unfold.
+    reflexivity.
+  }
+  follow10 LOverflow_0.
+  cbn.
+  repeat rewrite <-const_unfold.
+  finish.
+Qed.
+
+Lemma LC_Overflow_1' n:
+  pow2' n <> xH ->
+  (exists k0,
+  LC (pow2' n) <| RC 1 -->+
+  LC k0 |> RC 0 /\
+  ((pow2 n)*2 <= k0 < ((pow2 n)+1)*2)%positive
+  ).
+Proof.
+  intro H.
+  destruct n as [|n].
+  1: cbn in H; lia.
+  replace (S n) with (n+1) by lia.
+  destruct (LC_shl (pow2 (n+1)) [v0]) as [k0 [H0 H1]].
+  cbn in H0,H1.
+  rewrite app_nil_r in H0.
+  exists k0.
+  split.
+  - rewrite <-H0.
+    unfold LC.
+    rewrite Counter_pow2,Counter_pow2'.
+    replace (RC 1) with (rd1 *> const 0). 2:{
+      cbn.
+      repeat rewrite <-const_unfold.
+      reflexivity.
+    }
+    follow10 LOverflow_1.
+    replace (RC 0) with ([0;0;0]*>const 0). 2:{
+      cbn.
+      repeat rewrite <-const_unfold.
+      reflexivity.
+    }
+    finish.
+  - lia.
+Qed.
+
+Lemma LC_Overflow_0 n m:
+  pow2' n <> xH ->
+  LC (pow2' n) <| RC (Npos (m~0)) -->+
+  LC (pow2 n) |> RC0 ((pow2 (ctz m))~1) (shr m (S (ctz m))).
+Proof.
+  intro H.
+  destruct n as [|n].
+  1: cbn in H; lia.
+  replace (S n) with (n+1) by lia.
+  unfold LC.
+  rewrite Counter_pow2,Counter_pow2'.
+  unfold RC.
+  rewrite BinaryCounter_0_d0.
+  follow10 LOverflow_0.
+  unfold RC0,RC.
+  cbn[BinaryCounter].
+  rewrite Counter_pow2.
+  rewrite rotate_0.
+  rewrite <-Counter_shr_S_ctz; auto.
+Qed.
+
+Lemma LC_Overflow_1 n m:
+  pow2' n <> xH ->
+  (exists k0,
+  LC (pow2' n) <| RC (Npos (m~1)) -->+
+  LC k0 |> RC2 (pow2 (ctz m)) (shr m (S (ctz m))) /\
+  (pow2 n)*2 <= k0 < ((pow2 n)+1)*2)%positive.
+Proof.
+  intro H.
+  destruct n as [|n].
+  1: cbn in H; lia.
+  replace (S n) with (n+1) by lia.
+  destruct (LC_shl (pow2 (n+1)) [v0]) as [k0 [H0 H1]].
+  cbn in H0,H1.
+  rewrite app_nil_r in H0.
+  exists k0.
+  split.
+  - rewrite <-H0.
+    unfold LC.
+    rewrite Counter_pow2,Counter_pow2'.
+    unfold RC.
+    rewrite BinaryCounter_0_d1.
+    follow10 LOverflow_1.
+    unfold RC2,RC.
+    cbn[BinaryCounter].
+    rewrite Counter_pow2.
+    rewrite rotate_000.
+    rewrite <-Counter_shr_S_ctz; auto.
+  - apply H1.
+Qed.
+
+Lemma RC_Inc n l:
+  l |> RC n -->+
+  l <| RC (N.succ n).
+Proof.
+  apply BinaryCounter.RInc_0; auto.
+  - intros. apply RInc.
+  - cbv; (repeat rewrite <-const_unfold); reflexivity.
+Qed.
+
+Lemma RC0_Inc n m (Hnf:not_full n) l:
+  l |> RC0 n m -->+
+  l <| RC0 (Pos.succ n) m.
+Proof.
+  apply BinaryCounter.RInc; auto.
+  intros. apply RInc.
+Qed.
+
+Lemma RC0_Overflow n m l:
+  l |> RC0 (pow2' n) m -->+
+  l <| RC1 (pow2 n) m.
+Proof.
+  unfold RC0,RC1.
+  rewrite Counter_pow2,Counter_pow2'.
+  apply RInc.
+Qed.
+
+Lemma RC1_Inc n m (Hnf:not_full n) l:
+  l |> RC1 n m -->+
+  l <| RC1 (Pos.succ n) m.
+Proof.
+  apply BinaryCounter.RInc; auto.
+  intros. apply RInc.
+Qed.
+
+Lemma RC1_Overflow_0 k n:
+  (exists k0,
+  LC k |> RC1 (pow2' n) N0 -->+
+  LC k0 |> RC N0 /\
+  k*(pow2 (n*2+1)) <= k0 < (k+1)*(pow2 (n*2+1)))%positive.
+Proof.
+  destruct (LC_shl k (ls3 ++ ls4 ^^ n ++ ls5)) as [k0 [H0 H1]].
+  exists k0.
+  split.
+  - unfold RC1.
+    rewrite Counter_pow2'.
+    change ([1] *> rd1 *> RC N0) with ([1;1] *> [0;0;0] *> RC N0).
+    follow10 ROverflow_11.
+    rewrite H0.
+    cbn.
+    repeat rewrite <-const_unfold.
+    finish.
+  - replace (n * 2 + 1) with (length (ls3 ++ ls4 ^^ n ++ ls5)).
+    + apply H1.
+    + repeat rewrite app_length.
+      rewrite lpow_length.
+      lia.
+Qed.
+
+Lemma RC1_Overflow k n m:
+  (exists k0,
+  LC k |> RC1 (pow2' n) (Npos m) -->+
+  LC k0 |> RC2 (pow2 (ctz m)) (shr m (S (ctz m))) /\
+  k*(pow2 (n*2+1)) <= k0 < (k+1)*(pow2 (n*2+1)))%positive.
+Proof.
+  destruct (LC_shl k (ls3 ++ ls4 ^^ n ++ ls5)) as [k0 [H0 H1]].
+  exists k0.
+  split.
+  - unfold RC1,RC2.
+    rewrite Counter_pow2,Counter_pow2'.
+    change ([1] *> rd1 *> RC (N.pos m)) with ([1;1] *> [0;0;0] *> RC (N.pos m)).
+    follow10 ROverflow_11.
+    rewrite rotate_000.
+    unfold RC.
+    rewrite <-Counter_shr_S_ctz; auto.
+    rewrite H0.
+    finish.
+  - replace (n * 2 + 1) with (length (ls3 ++ ls4 ^^ n ++ ls5)).
+    + apply H1.
+    + repeat rewrite app_length.
+      rewrite lpow_length.
+      lia.
+Qed.
+
+Lemma RC2_Inc n m (Hnf:not_full n) l:
+  l |> RC2 n m -->+
+  l <| RC2 (Pos.succ n) m.
+Proof.
+  apply BinaryCounter.RInc; auto.
+  intros. apply RInc.
+Qed.
+
+Lemma RC2_Overflow n m l:
+  l |> RC2 (pow2' n) m -->+
+  l <| RC3 (pow2 n) m.
+Proof.
+  unfold RC2,RC3.
+  rewrite Counter_pow2,Counter_pow2'.
+  apply RInc.
+Qed.
+
+Lemma RC3_Inc n m (Hnf:not_full n) l:
+  l |> RC3 n m -->+
+  l <| RC3 (Pos.succ n) m.
+Proof.
+  apply BinaryCounter.RInc; auto.
+  intros. apply RInc.
+Qed.
+
+Lemma RC3_Overflow_0 k n:
+  (exists k0,
+  LC k |> RC3 (pow2' n) N0 -->+
+  LC k0 |> RC N0 /\
+  k*(pow2 (n*2+2)) <= k0 < (k+1)*(pow2 (n*2+2)))%positive.
+Proof.
+  destruct (LC_shl k (ls0 ++ ls1 ^^ n ++ ls2)) as [k0 [H0 H1]].
+  exists k0.
+  split.
+  - unfold RC3.
+    rewrite Counter_pow2'.
+    change ([1;0;0] *> rd1 *> RC N0) with ([1;0;0;1] *> [0;0;0] *> RC N0).
+    follow10 ROverflow_1001.
+    rewrite H0.
+    cbn.
+    repeat rewrite <-const_unfold.
+    finish.
+  - replace (n * 2 + 2) with (length (ls0 ++ ls1 ^^ n ++ ls2)).
+    + apply H1.
+    + repeat rewrite app_length.
+      rewrite lpow_length.
+      lia.
+Qed.
+
+Lemma RC3_Overflow k n m:
+  (exists k0,
+  LC k |> RC3 (pow2' n) (Npos m) -->+
+  LC k0 |> RC2 (pow2 (ctz m)) (shr m (S (ctz m))) /\
+  k*(pow2 (n*2+2)) <= k0 < (k+1)*(pow2 (n*2+2)))%positive.
+Proof.
+  destruct (LC_shl k (ls0 ++ ls1 ^^ n ++ ls2)) as [k0 [H0 H1]].
+  exists k0.
+  split.
+  - unfold RC3,RC2.
+    rewrite Counter_pow2,Counter_pow2'.
+    change ([1;0;0] *> rd1 *> RC (N.pos m)) with ([1;0;0;1] *> [0;0;0] *> RC (N.pos m)).
+    follow10 ROverflow_1001.
+    rewrite rotate_000.
+    unfold RC.
+    rewrite <-Counter_shr_S_ctz; auto.
+    rewrite H0.
+    finish.
+  - replace (n * 2 + 2) with (length (ls0 ++ ls1 ^^ n ++ ls2)).
+    + apply H1.
+    + repeat rewrite app_length.
+      rewrite lpow_length.
+      lia.
+Qed.
+
+
+
+
+Inductive Config :=
+| cfgL(k:positive)(n:N)
+| cfgR(k:positive)(n:N)
+| cfg0L(k n:positive)(m:N)
+| cfg0R(k n:positive)(m:N)
+| cfg1L(k n:positive)(m:N)
+| cfg1R(k n:positive)(m:N)
+| cfg2L(k n:positive)(m:N)
+| cfg2R(k n:positive)(m:N)
+| cfg3L(k n:positive)(m:N)
+| cfg3R(k n:positive)(m:N)
+.
+
+
+
+Definition to_config(x:Config):=
+match x with
+| cfgL k n => LC k <| RC n
+| cfgR k n => LC k |> RC n
+| cfg0L k n m => LC k <| RC0 n m
+| cfg0R k n m => LC k |> RC0 n m
+| cfg1L k n m => LC k <| RC1 n m
+| cfg1R k n m => LC k |> RC1 n m
+| cfg2L k n m => LC k <| RC2 n m
+| cfg2R k n m => LC k |> RC2 n m
+| cfg3L k n m => LC k <| RC3 n m
+| cfg3R k n m => LC k |> RC3 n m
+end.
+
+Definition P(x:Config):Prop :=
+(match x with
+| cfgL k n => k<>xH /\ rest (pow2 (log2 k)) >= n + rest k + 0 /\ n + rest k >= 2
+| cfgR k n => k<>xH /\ rest (pow2 (log2 k)) >= n + rest k + 1 /\ n + rest k >= 1
+| cfg0L k n m => rest n + m + rest (pow2 (log2 n)) + 3 <= rest k
+| cfg0R k n m => rest n + m + rest (pow2 (log2 n)) + 2 <= rest k
+| cfg1L k n m => rest n + m + 2 <= rest k
+| cfg1R k n m => rest n + m + 1 <= rest k < rest (pow2 (log2 k))
+| cfg2L k n m => rest n + m + rest (pow2 (log2 n)) + 3 <= rest k
+| cfg2R k n m => rest n + m + rest (pow2 (log2 n)) + 2 <= rest k
+| cfg3L k n m => rest n + m + 2 <= rest k
+| cfg3R k n m => rest n + m + 1 <= rest k < rest (pow2 (log2 k))
+end)%N.
+
+Hypothesis init: c0 -->* to_config (cfgL k_init n_init).
+Hypothesis P_init: P (cfgL k_init n_init).
+
+
+
+Lemma nonhalt: ~halts tm c0.
+Proof.
+apply multistep_nonhalt with (c':=to_config (cfgL k_init n_init)).
+1: apply init.
+apply (progress_nonhalt_cond tm _ _ _ P).
+2: apply P_init.
+intros i H.
+destruct i.
+- cbn[to_config].
+  destruct H as [H0 H1].
+  destruct (full_cases k) as [E|E].
+  + destruct n as [|[n|n|]].
+    * rewrite full_iff_rest in E. lia.
+    * epose proof (LC_Overflow_1 (log2 k) n _) as H2.
+      destruct H2 as [k0 [H2 H3]].
+      exists (cfg2R k0 (pow2 (ctz n)) (shr n (S (ctz n)))). split.
+      -- rewrite full_iff_pow2' in E.
+        rewrite E.
+        apply H2.
+      -- cbn[P].
+        destruct (rest_pow2_add _ 1 _ H3) as [H3' H3''].
+        pose proof (le_pow2a _ _ 0 0 H3').
+        rewrite log2_pow2.
+        pose proof (split_bound n). lia.
+    * epose proof (LC_Overflow_0 (log2 k) n _) as H2.
+      rewrite full_iff_pow2' in E.
+      rewrite E.
+      eexists (cfg0R _ _ _). split.
+      -- apply H2.
+      -- cbn[P].
+        cbn[log2].
+        rewrite log2_pow2.
+        rewrite rest_mul2add1.
+        pose proof (rest_pow2 (ctz n)) as E1.
+        pose proof (rest_pow2 (S (ctz n))) as E2.
+        cbn[pow2] in E2. cbn[pow2].
+        pose proof (rest_pow2 (log2 k)) as E3.
+        assert (2 <= n*2 < pow2 (log2 k))%positive as E4 by lia.
+        pose proof (split_bound' _ _ E4).
+        lia.
+    * rewrite full_iff_rest in E. lia.
+  + exists (cfgR (Pos.succ k) n). split.
+    * cbn[to_config].
+      apply LC_Inc,E.
+    * cbn[P].
+      rewrite not_full_log2_S; auto.
+      rewrite not_full_iff_rest in E.
+      rewrite <-(rest_S k) in H1; auto.
+      lia.
+- cbn[to_config].
+  cbn[P] in H.
+  exists (cfgL k (N.succ n)). split.
+  + apply RC_Inc.
+  + cbn[P].
+    lia.
+- cbn[to_config].
+  cbn[P] in H.
+  assert (rest k <> 0%N) as E by (lia).
+  rewrite <-not_full_iff_rest in E.
+  exists (cfg0R (Pos.succ k) n m). split.
+  + apply (LC_Inc _ E).
+  + cbn[P].
+    rewrite not_full_iff_rest in E.
+    rewrite <-(rest_S k) in H; auto. lia.
+- cbn[to_config].
+  cbn[P] in H.
+  destruct (full_cases n) as [E0|E0].
+  + eexists (cfg1L k (pow2 (log2 n)) m). split.
+    * rewrite full_iff_pow2' in E0.
+      rewrite E0.
+      cbn[to_config].
+      follow10 (RC0_Overflow).
+      rewrite <-E0.
+      finish.
+    * cbn[P]. lia.
+  + eexists (cfg0L k (Pos.succ n) m). split.
+    * apply (RC0_Inc n m E0).
+    * cbn[P].
+      rewrite not_full_log2_S; auto.
+      rewrite not_full_iff_rest in E0.
+      rewrite <-(rest_S n) in H; auto. lia.
+- cbn[to_config].
+  cbn[P] in H.
+  assert (rest k <> 0%N) as E by lia.
+  rewrite <-not_full_iff_rest in E.
+  exists (cfg1R (Pos.succ k) n m). split.
+  + apply LC_Inc,E.
+  + cbn[P].
+    rewrite not_full_iff_rest in E.
+    rewrite <-(rest_S k) in H; auto. split; try lia.
+    apply rest_S_not_empty,E.
+- cbn[to_config].
+  cbn[P] in H.
+  destruct (full_cases n) as [E0|E0].
+  + rewrite full_iff_pow2' in E0.
+    rewrite E0.
+    destruct m as [|m].
+    * destruct (RC1_Overflow_0 k (log2 n)) as [k0 [H2 H3]].
+      eexists (cfgR k0 0). split.
+      -- apply H2.
+      -- cbn[P].
+        pose proof (not_empty_rest_pow2_add _ _ _ H3).
+        repeat split; try lia.
+        destruct (rest_pow2_add _ _ _ H3) as [H1 _].
+        epose proof (N.mul_le_mono_l 1 (N.pos (pow2 (log2 n * 2 + 1))) (rest k)).
+        lia.
+    * destruct (RC1_Overflow k (log2 n) m) as [k0 [H2 H3]].
+      eexists (cfg2R k0 _ _). split.
+      -- follow10 H2. finish.
+      -- cbn[P].
+        destruct (rest_pow2_add _ _ _ H3) as [H3' H3''].
+        pose proof (le_pow2a _ _ _ _ H3').
+        rewrite log2_pow2.
+        pose proof (split_bound m). lia.
+  + eexists (cfg1L _ _ _). split.
+    * apply (RC1_Inc n m E0).
+    * cbn[P].
+      rewrite not_full_iff_rest in E0.
+      rewrite <-(rest_S n) in H; auto. lia.
+- cbn[to_config].
+  cbn[P] in H.
+  assert (rest k <> 0%N) as E by lia.
+  rewrite <-not_full_iff_rest in E.
+  eexists (cfg2R _ _ _). split.
+  + apply LC_Inc,E.
+  + cbn[P].
+    rewrite not_full_iff_rest in E.
+    rewrite <-(rest_S k) in H; auto. lia.
+- cbn[to_config].
+  cbn[P] in H.
+  destruct (full_cases n) as [E0|E0].
+  + rewrite full_iff_pow2' in E0.
+    rewrite E0.
+    eexists (cfg3L _ _ _). split.
+    * apply RC2_Overflow.
+    * cbn[P]. lia.
+  + eexists (cfg2L _ _ _). split.
+    * apply RC2_Inc,E0.
+    * cbn[P].
+      rewrite not_full_log2_S; auto.
+      rewrite not_full_iff_rest in E0.
+      rewrite <-(rest_S n) in H; auto. lia.
+- cbn[to_config].
+  cbn[P] in H.
+  assert (rest k <> 0%N) as E by lia.
+  rewrite <-not_full_iff_rest in E.
+  eexists (cfg3R _ _ _). split.
+  + apply LC_Inc,E.
+  + cbn[P].
+    rewrite not_full_iff_rest in E.
+    rewrite <-(rest_S k) in H; auto.
+    split. 1: lia.
+    apply rest_S_not_empty,E.
+- cbn[to_config].
+  cbn[P] in H.
+  destruct (full_cases n) as [E0|E0].
+  + rewrite full_iff_pow2' in E0.
+    rewrite E0.
+    destruct m as [|m].
+    * destruct (RC3_Overflow_0 k (log2 n)) as [k0 [H2 H3]].
+      eexists (cfgR k0 0). split.
+      -- apply H2.
+      -- cbn[P].
+        epose proof (not_empty_rest_pow2_add _ _ _ H3).
+        destruct (rest_pow2_add _ _ _ H3) as [H1 _].
+        epose proof (N.mul_le_mono_l 1 (N.pos (pow2 (log2 n * 2 + 1))) (rest k)).
+        lia.
+    * destruct (RC3_Overflow k (log2 n) m) as [k0 [H2 H3]].
+      eexists (cfg2R k0 _ _). split.
+      -- follow10 H2. finish.
+      -- cbn[P].
+        destruct (rest_pow2_add _ _ _ H3) as [H3' H3''].
+        pose proof (le_pow2a _ _ _ _ H3').
+        rewrite log2_pow2.
+        pose proof (split_bound m). lia.
+  + eexists (cfg3L _ _ _). split.
+    * apply (RC3_Inc n m E0).
+    * cbn[P].
+      rewrite not_full_iff_rest in E0.
+      rewrite <-(rest_S n) in H; auto. lia.
+Unshelve.
+all: destruct k; cbn in H0; cbn; lia.
+Qed.
+
+End SOCv1.
+
+
+
+
+
+Inductive SOC_cert_v1 :=
+| Build_SOC_cert_v1
+  (QL QR : Q)
+  (qL qR : list Sym)
+  (v0 : nat)
+  (ls0 ls1 ls2 ls3 ls4 ls5: list nat)
+  (k_init: positive)
+  (n_init : N).
+
+Ltac solve_LOverflow :=
+  intros;
+  simpl_tape; cbn; step1s;
+  use_shift_rule; cbn;
+  step1s;
+  use_shift_rule; cbn;
+  simpl_rotate;
+  step1s.
+
+Ltac solve_SOCv1 tm cert :=
+match cert with
+  (Build_SOC_cert_v1
+  ?QL ?QR
+  ?qL ?qR
+  ?v0
+  ?ls0 ?ls1 ?ls2 ?ls3 ?ls4 ?ls5
+  ?k_init
+  ?n_init) =>
+  eapply (nonhalt tm
+    QL QR
+    qL qR
+    v0
+    ls0 ls1 ls2 ls3 ls4 ls5
+    k_init n_init);
+  [ try (intros l r n; casen_execute_with_shift_rule n; fail)
+  | try (intros l r n; casen_execute_with_shift_rule n; fail)
+  | try (solve_LOverflow; fail)
+  | try (solve_LOverflow; fail)
+  | reflexivity
+  | reflexivity
+  | reflexivity
+  | reflexivity
+  | try (intros l r n;
+    simpl_flat_map;
+    casen_execute_with_shift_rule n;
+    fail)
+  | try (intros l r n;
+    simpl_flat_map;
+    casen_execute_with_shift_rule n;
+    fail)
+  | try (cbn; solve_init; fail)
+  | try (cbn; lia; fail)
+  ]
+end.
+
+
+
+
+
+
+
+
